Refinery/Ctx/SSplit.lean
@@ -1,0 +1,718 @@
+import Refinery.Ctx.Basic
+
+namespace Refinery
+
+variable [HasQuant α]
+
+open HasQuant
+
+inductive Var?.SSplit : Var? α ε → Var? α ε → Var? α ε → Type _
+  | left (v) : SSplit v v v.erase
+  | right (v) : SSplit v v.erase v
+  | sboth {v} : v.scopy → SSplit v v v
+
+theorem Var?.SSplit.left_unused {u v w : Var? α ε} (σ : u.SSplit v w) (h : u.unused) : v.unused
+  := by cases σ <;> first | assumption | rfl
+
+theorem Var?.SSplit.right_unused {u v w : Var? α ε} (σ : u.SSplit v w) (h : u.unused) : w.unused
+  := by cases σ <;> first | rfl | assumption
+
+theorem Var?.SSplit.used_of_left {u v w : Var? α ε} (σ : u.SSplit v w) (h : v.used) : u.used
+  := by cases σ <;> first | assumption | cases h
+
+theorem Var?.SSplit.used_of_right {u v w : Var? α ε} (σ : u.SSplit v w) (h : w.used) : u.used
+  := by cases σ <;> first | cases h | assumption
+
+theorem Var?.SSplit.erase_eq_left {u v w : Var? α ε} (h : u.SSplit v w)
+  : u.erase = v.erase := by cases h <;> simp [*]
+
+theorem Var?.SSplit.erase_eq_right {u v w : Var? α ε} (h : u.SSplit v w)
+  : u.erase = w.erase := by cases h <;> simp [*]
+
+theorem Var?.SSplit.erase_eq_both {u v w : Var? α ε} (h : u.SSplit v w)
+  : v.erase = w.erase := by cases h <;> simp [*]
+
+def Var?.SSplit.both (v : Var? α ε) [h : IsRel v] : SSplit v v v := if hv : v.used then
+    SSplit.sboth hv.scopy
+  else by
+    rw [<-Var?.unused_iff] at hv
+    convert SSplit.left v
+    rw [hv.eq_erase]
+
+def Var?.SSplit.wkLeft {u v w : Var? α ε} (u' : Var? α ε)
+  : u.SSplit v w → Var? α ε
+  | .left _ => if u.used then u' else u'.erase
+  | .right _ => u'.erase
+  | .sboth _ => if u.used then u' else u'.erase
+
+@[simp]
+theorem Var?.SSplit.wkLeft_left {u' u : Var? α ε}
+  : (SSplit.left u).wkLeft u' = if u.used then u' else u'.erase := rfl
+
+@[simp]
+theorem Var?.SSplit.wkLeft_right {u' u : Var? α ε}
+  : (SSplit.right u).wkLeft u' = u'.erase := rfl
+
+@[simp]
+theorem Var?.SSplit.wkLeft_sboth {u' u : Var? α ε} (h : u.scopy)
+  : (SSplit.sboth h).wkLeft u' = if u.used then u' else u'.erase := rfl
+
+def Var?.SSplit.wkRight {u v w : Var? α ε} (u' : Var? α ε)
+  : u.SSplit v w → Var? α ε
+  | .left _ => if u.used then u'.erase else u'
+  | .right _ => u'
+  | .sboth _ => u'
+
+@[simp]
+theorem Var?.SSplit.wkRight_left {u' u : Var? α ε}
+  : (SSplit.left u).wkRight u' = if u.used then u'.erase else u' := rfl
+
+@[simp]
+theorem Var?.SSplit.wkRight_right {u' u : Var? α ε}
+  : (SSplit.right u).wkRight u' = u' := rfl
+
+@[simp]
+theorem Var?.SSplit.wkRight_sboth {u' u : Var? α ε} (h : u.scopy)
+  : (SSplit.sboth h).wkRight u' = u' := rfl
+
+def Var?.SSplit.wkLeft' {u v w : Var? α ε} (u' : Var? α ε)
+  : u.SSplit v w → Var? α ε
+  | .left _ => u'
+  | .right _ => if u.used then u'.erase else u'
+  | .sboth _ => u'
+
+@[simp]
+theorem Var?.SSplit.wkLeft_left' {u' u : Var? α ε}
+  : (SSplit.left u).wkLeft' u' = u' := rfl
+
+@[simp]
+theorem Var?.SSplit.wkLeft_right' {u' u : Var? α ε}
+  : (SSplit.right u).wkLeft' u' = if u.used then u'.erase else u' := rfl
+
+@[simp]
+theorem Var?.SSplit.wkLeft_sboth' {u' u : Var? α ε} (h : u.scopy)
+  : (SSplit.sboth h).wkLeft' u' = u' := rfl
+
+def Var?.SSplit.wkRight' {u v w : Var? α ε} (u' : Var? α ε)
+  : u.SSplit v w → Var? α ε
+  | .left _ => u'.erase
+  | .right _ => if u.used then u' else u'.erase
+  | .sboth _ => if u.used then u' else u'.erase
+
+@[simp]
+theorem Var?.SSplit.wkRight_left' {u' u : Var? α ε}
+  : (SSplit.left u).wkRight' u' = u'.erase := rfl
+
+@[simp]
+theorem Var?.SSplit.wkRight_right' {u' u : Var? α ε}
+  : (SSplit.right u).wkRight' u' = if u.used then u' else u'.erase := rfl
+
+@[simp]
+theorem Var?.SSplit.wkRight_sboth' {u' u : Var? α ε} (h : u.scopy)
+  : (SSplit.sboth h).wkRight' u' = if u.used then u' else u'.erase := rfl
+
+theorem Var?.SSplit.left_ty_eq {u v w : Var? α ε} (h : u.SSplit v w) : u.ty = v.ty
+  := by cases h <;> rfl
+
+theorem Var?.SSplit.right_ty_eq {u v w : Var? α ε} (h : u.SSplit v w) : u.ty = w.ty
+  := by cases h <;> rfl
+
+theorem Var?.SSplit.left_eff_eq {u v w : Var? α ε} (h : u.SSplit v w) : u.eff = v.eff
+  := by cases h <;> rfl
+
+theorem Var?.SSplit.right_eff_eq {u v w : Var? α ε} (h : u.SSplit v w) : u.eff = w.eff
+  := by cases h <;> rfl
+
+theorem Var?.SSplit.left_eq_erase {u v w : Var? α ε} (h : u.SSplit v w) (hv : v.unused)
+  : v = u.erase := by cases u; cases h <;> cases hv <;> rfl
+
+theorem Var?.SSplit.right_eq_of_left {u v w : Var? α ε} (h : u.SSplit v w) (hv : v.unused)
+  : w = u := by cases u; cases h <;> cases hv <;> rfl
+
+theorem Var?.SSplit.right_eq_erase {u v w : Var? α ε} (h : u.SSplit v w) (hw : w.unused)
+  : w = u.erase := by cases u; cases h <;> cases hw <;> rfl
+
+theorem Var?.SSplit.left_eq {u v w : Var? α ε} (h : u.SSplit v w) (hv : v.used)
+  : v = u := by cases h <;> first | rfl | cases hv
+
+theorem Var?.SSplit.right_eq {u v w : Var? α ε} (h : u.SSplit v w) (hw : w.used)
+  : w = u := by cases h <;> first | rfl | cases hw
+
+theorem Var?.SSplit.scopy {u v w : Var? α ε}
+  (h : u.SSplit v w) (hv : v.used) (hw : w.used) : u.scopy
+  := by cases h <;> first | cases hv | cases hw | assumption
+
+def Var?.SSplit.cast {u v w u' v' w' : Var? α ε}
+  (h : u.SSplit v w) (hu : u = u') (hv : v = v') (hw : w = w')
+  : u'.SSplit v' w' := hu ▸ hv ▸ hw ▸ h
+
+def Var?.SSplit.choose {u v w : Var? α ε} (h : Nonempty (u.SSplit v w)) : u.SSplit v w
+  := if hv : v.used then
+      have ev := Eq.symm <| let ⟨h⟩ := h; h.left_eq hv;
+      if hw : w.used then
+        have ew := Eq.symm <| let ⟨h⟩ := h; h.right_eq hw;
+        have hc := let ⟨h⟩ := h; h.scopy hv hw;
+        (Var?.SSplit.sboth hc).cast rfl ev ew
+      else
+        have ew := Eq.symm <| let ⟨h⟩ := h; h.right_eq_erase (unused_iff.mpr hw);
+        (Var?.SSplit.left u).cast rfl ev ew
+    else
+      have ev := Eq.symm <| let ⟨h⟩ := h; h.left_eq_erase (Var?.unused_iff.mpr hv);
+      have ew := Eq.symm <| let ⟨h⟩ := h; h.right_eq_of_left (Var?.unused_iff.mpr hv);
+      (Var?.SSplit.right u).cast rfl ev ew
+
+inductive Ctx?.SSplit : Ctx? α ε → Ctx? α ε → Ctx? α ε → Type _ where
+  | nil : Ctx?.SSplit .nil .nil .nil
+  | cons {Γ Δ Ξ v l r} (h : SSplit Γ Δ Ξ) (hvw : v.SSplit l r)
+    : SSplit (Ctx?.cons Γ v) (Ctx?.cons Δ l) (Ctx?.cons Ξ r)
+
+def Ctx?.SSplit.choose {Γ Δ Ξ : Ctx? α ε} (h : Nonempty (Ctx?.SSplit Γ Δ Ξ)) : Ctx?.SSplit Γ Δ Ξ
+  := match Γ, Δ, Ξ, h with
+  | .nil, .nil, .nil, h => .nil
+  | .nil, .cons _ _, _, h => False.elim (let ⟨h⟩ := h; by cases h)
+  | .nil, _, .cons _ _, h => False.elim (let ⟨h⟩ := h; by cases h)
+  | .cons _ _, .nil, _, h => False.elim (let ⟨h⟩ := h; by cases h)
+  | .cons _ _, _, .nil, h => False.elim (let ⟨h⟩ := h; by cases h)
+  | .cons Γ v, .cons Δ l, .cons Ξ r, h =>
+    .cons (choose (let ⟨h⟩ := h; ⟨by cases h; assumption⟩))
+          (Var?.SSplit.choose (let ⟨h⟩ := h; ⟨by cases h; assumption⟩))
+
+theorem Ctx?.SSplit.left_length {Γ Δ Ξ : Ctx? α ε} (h : Ctx?.SSplit Γ Δ Ξ)
+  : Ctx?.length Γ = Ctx?.length Δ
+  := by induction h <;> simp [*]
+
+theorem Ctx?.SSplit.right_length {Γ Δ Ξ : Ctx? α ε} (h : Ctx?.SSplit Γ Δ Ξ)
+  : Ctx?.length Γ = Ctx?.length Ξ
+  := by induction h <;> simp [*]
+
+theorem Ctx?.SSplit.target_length {Γ Δ Ξ : Ctx? α ε} (h : Ctx?.SSplit Γ Δ Ξ)
+  : Ctx?.length Δ = Ctx?.length Ξ := h.left_length.symm.trans h.right_length
+
+def Ctx?.both (Γ : Ctx? α ε) [hΓ : Γ.copy] : Γ.SSplit Γ Γ := (λ_ => match Γ with
+  | .nil => .nil
+  | .cons Γ v => .cons (have _ := copy.tail Γ v; Γ.both) (have _ := copy.head Γ v; .both v)) hΓ
+
+def Var?.SSplit.comm {u v w : Var? α ε} : u.SSplit v w → u.SSplit w v
+  | .left _ => .right _
+  | .right _ => .left _
+  | .sboth h => .sboth h
+
+def Var?.SSplit.v12_3_23 {u₁₂₃ u₁₂ u₁ u₂ u₃ : Var? α ε}
+  : u₁₂₃.SSplit u₁₂ u₃ → u₁₂.SSplit u₁ u₂ → Var? α ε
+  | .left _, .left _ => u₁₂₃.erase
+  | _, _ => u₁₂₃
+
+def Var?.SSplit.s12_3_1_23 {u₁₂₃ u₁₂ u₁ u₂ u₃ : Var? α ε}
+  : (h12_3 : u₁₂₃.SSplit u₁₂ u₃) → (h12 : u₁₂.SSplit u₁ u₂) → u₁₂₃.SSplit u₁ (h12_3.v12_3_23 h12)
+  | .left _, .left _ => .left _
+  | .left _, .right _ => .right _
+  | .left _, .sboth h => .sboth h
+  | .right _, .left _ => .right _
+  | .right _, .right _ => .right _
+  | .right _, .sboth _ => .right _
+  | .sboth h, .left _ => .sboth h
+  | .sboth _, .right _ => .right _
+  | .sboth h, .sboth _ => .sboth h
+
+def Var?.SSplit.s12_3_23 {u₁₂₃ u₁₂ u₁ u₂ u₃ : Var? α ε}
+  : (h12_3 : u₁₂₃.SSplit u₁₂ u₃) → (h12 : u₁₂.SSplit u₁ u₂) → (h12_3.v12_3_23 h12).SSplit u₂ u₃
+  | .left _, .left _ => .left _
+  | .left _, .right _ => .left _
+  | .left _, .sboth _ => .left _
+  | .right _, .left _ => .right _
+  | .right _, .right _ => .right _
+  | .right _, .sboth _ => .right _
+  | .sboth _, .left _ => .right _
+  | .sboth h, .right _ => .sboth h
+  | .sboth h, .sboth _ => .sboth h
+
+def Var?.SSplit.v1_23_12 {u₁₂₃ u₂₃ u₁ u₂ u₃ : Var? α ε}
+  : u₁₂₃.SSplit u₁ u₂₃ → u₂₃.SSplit u₂ u₃ → Var? α ε
+  | .right _, .right _ => u₁₂₃.erase
+  | _, _ => u₁₂₃
+
+def Var?.SSplit.s1_23_12_3 {u₁₂₃ u₂₃ u₁ u₂ u₃ : Var? α ε}
+  : (h12_3 : u₁₂₃.SSplit u₁ u₂₃) → (h23 : u₂₃.SSplit u₂ u₃) → u₁₂₃.SSplit (h12_3.v1_23_12 h23) u₃
+  | .left _, .left _ => .left _
+  | .left _, .right _ => .left _
+  | .left _, .sboth _ => .left _
+  | .right _, .left _ => .left _
+  | .right _, .right _ => .right _
+  | .right _, .sboth h => .sboth h
+  | .sboth _, .left _ => .left _
+  | .sboth h, .right _ => .sboth h
+  | .sboth h, .sboth _ => .sboth h
+
+def Var?.SSplit.s1_23_12 {u₁₂₃ u₂₃ u₁ u₂ u₃ : Var? α ε}
+  : (h12_3 : u₁₂₃.SSplit u₁ u₂₃) → (h23 : u₂₃.SSplit u₂ u₃) → (h12_3.v1_23_12 h23).SSplit u₁ u₂
+  | .left _, .left _ => .left _
+  | .left _, .right _ => .left _
+  | .left _, .sboth h => .left _
+  | .right _, .left _ => .right _
+  | .right _, .right _ => .right _
+  | .right _, .sboth _ => .right _
+  | .sboth h, .left _ => .sboth h
+  | .sboth h, .right _ => .left _
+  | .sboth h, .sboth _ => .sboth h
+
+def Ctx?.SSplit.comm {Γ Δ Ξ : Ctx? α ε} : Γ.SSplit Δ Ξ → Γ.SSplit Ξ Δ
+  | .nil => .nil
+  | .cons h hvw => .cons (SSplit.comm h) hvw.comm
+
+def Ctx?.SSplit.c1_23_12 {Γ₁₂₃ Γ₂₃ Γ₁ Γ₂ Γ₃ : Ctx? α ε}
+  : Γ₁₂₃.SSplit Γ₁ Γ₂₃ → Γ₂₃.SSplit Γ₂ Γ₃ → Ctx? α ε
+  | .nil, .nil => .nil
+  | .cons h hvw, .cons h' hvw' => .cons (c1_23_12 h h') (Var?.SSplit.v1_23_12 hvw hvw')
+
+def Ctx?.SSplit.s1_23_12_3 {Γ₁₂₃ Γ₂₃ Γ₁ Γ₂ Γ₃ : Ctx? α ε}
+  : (h12_3 : Γ₁₂₃.SSplit Γ₁ Γ₂₃) → (h23 : Γ₂₃.SSplit Γ₂ Γ₃)
+    → Γ₁₂₃.SSplit (h12_3.c1_23_12 h23) Γ₃
+  | .nil, .nil => .nil
+  | .cons h hvw, .cons h' hvw' => .cons (s1_23_12_3 h h') (Var?.SSplit.s1_23_12_3 hvw hvw')
+
+def Ctx?.SSplit.s1_23_12 {Γ₁₂₃ Γ₂₃ Γ₁ Γ₂ Γ₃ : Ctx? α ε}
+  : (h12_3 : Γ₁₂₃.SSplit Γ₁ Γ₂₃) → (h23 : Γ₂₃.SSplit Γ₂ Γ₃) → (h12_3.c1_23_12 h23).SSplit Γ₁ Γ₂
+  | .nil, .nil => .nil
+  | .cons h hvw, .cons h' hvw' => .cons (s1_23_12 h h') (Var?.SSplit.s1_23_12 hvw hvw')
+
+def Ctx?.SSplit.c12_3_23 {Γ₁₂₃ Γ₁₂ Γ₁ Γ₂ Γ₃ : Ctx? α ε}
+  : Γ₁₂₃.SSplit Γ₁₂ Γ₃ → Γ₁₂.SSplit Γ₁ Γ₂ → Ctx? α ε
+  | .nil, .nil => .nil
+  | .cons h hvw, .cons h' hvw' => .cons (c12_3_23 h h') (Var?.SSplit.v12_3_23 hvw hvw')
+
+def Ctx?.SSplit.s12_3_1_23 {Γ₁₂₃ Γ₁₂ Γ₁ Γ₂ Γ₃ : Ctx? α ε}
+  : (h12_3 : Γ₁₂₃.SSplit Γ₁₂ Γ₃) → (h12 : Γ₁₂.SSplit Γ₁ Γ₂)
+    → Γ₁₂₃.SSplit Γ₁ (h12_3.c12_3_23 h12)
+  | .nil, .nil => .nil
+  | .cons h hvw, .cons h' hvw' => .cons (s12_3_1_23 h h') (Var?.SSplit.s12_3_1_23 hvw hvw')
+
+def Ctx?.SSplit.s12_3_23 {Γ₁₂₃ Γ₁₂ Γ₁ Γ₂ Γ₃ : Ctx? α ε}
+  : (h12_3 : Γ₁₂₃.SSplit Γ₁₂ Γ₃) → (h12 : Γ₁₂.SSplit Γ₁ Γ₂) → (h12_3.c12_3_23 h12).SSplit Γ₂ Γ₃
+  | .nil, .nil => .nil
+  | .cons h hvw, .cons h' hvw' => .cons (s12_3_23 h h') (Var?.SSplit.s12_3_23 hvw hvw')
+
+theorem Ctx?.SSplit.erase_eq_left {Γ Δ Ξ : Ctx? α ε} (h : Γ.SSplit Δ Ξ)
+  : Γ.erase = Δ.erase := by induction h with
+  | nil => rfl
+  | cons h hvw I => simp [I, hvw.erase_eq_left]
+
+theorem Ctx?.SSplit.erase_eq_right {Γ Δ Ξ : Ctx? α ε} (h : Γ.SSplit Δ Ξ)
+  : Γ.erase = Ξ.erase := h.comm.erase_eq_left
+
+theorem Ctx?.SSplit.erase_eq {Γ Δ Ξ : Ctx? α ε} (h : Γ.SSplit Δ Ξ)
+  : Δ.erase = Ξ.erase := h.erase_eq_left.symm.trans h.erase_eq_right
+
+def Ctx?.SSplit.cast {Γ Δ Ξ Γ' Δ' Ξ' : Ctx? α ε}
+  (h : Γ.SSplit Δ Ξ) (hΓ : Γ = Γ') (hΔ : Δ = Δ') (hΞ : Ξ = Ξ')
+  : Γ'.SSplit Δ' Ξ' := hΓ ▸ hΔ ▸ hΞ ▸ h
+
+abbrev Ctx?.SSplit.cast_src {Γ Δ Ξ Γ' : Ctx? α ε}
+  (h : Γ.SSplit Δ Ξ) (hΓ : Γ = Γ')
+  : Γ'.SSplit Δ Ξ := h.cast hΓ rfl rfl
+
+abbrev Ctx?.SSplit.cast_left {Γ Δ Ξ Δ' : Ctx? α ε}
+  (h : Γ.SSplit Δ Ξ) (hΔ : Δ = Δ')
+  : Γ.SSplit Δ' Ξ := h.cast rfl hΔ rfl
+
+abbrev Ctx?.SSplit.cast_right {Γ Δ Ξ Ξ' : Ctx? α ε}
+  (h : Γ.SSplit Δ Ξ) (hΞ : Ξ = Ξ')
+  : Γ.SSplit Δ Ξ' := h.cast rfl rfl hΞ
+
+abbrev Ctx?.SSplit.c12_3_13 {Γ₁₂₃ Γ₁₂ Γ₁ Γ₂ Γ₃ : Ctx? α ε}
+  (h12_3 : Γ₁₂₃.SSplit Γ₁₂ Γ₃) (h12 : Γ₁₂.SSplit Γ₁ Γ₂)
+  : Ctx? α ε := h12_3.comm.c1_23_12 h12
+
+abbrev Ctx?.SSplit.s12_3_13_2 {Γ₁₂₃ Γ₁₂ Γ₁ Γ₂ Γ₃ : Ctx? α ε}
+  (h12_3 : Γ₁₂₃.SSplit Γ₁₂ Γ₃) (h12 : Γ₁₂.SSplit Γ₁ Γ₂)
+  : Γ₁₂₃.SSplit (h12_3.c12_3_13 h12) Γ₂
+  := h12_3.comm.s1_23_12_3 h12
+
+abbrev Ctx?.SSplit.s12_3_31 {Γ₁₂₃ Γ₁₂ Γ₁ Γ₂ Γ₃ : Ctx? α ε}
+  (h12_3 : Γ₁₂₃.SSplit Γ₁₂ Γ₃) (h12 : Γ₁₂.SSplit Γ₁ Γ₂)
+  : (h12_3.c12_3_13 h12).SSplit Γ₃ Γ₁
+  := h12_3.comm.s1_23_12 h12
+
+abbrev Ctx?.SSplit.s12_3_13 {Γ₁₂₃ Γ₁₂ Γ₁ Γ₂ Γ₃ : Ctx? α ε}
+  (h12_3 : Γ₁₂₃.SSplit Γ₁₂ Γ₃) (h12 : Γ₁₂.SSplit Γ₁ Γ₂)
+  : (h12_3.c12_3_13 h12).SSplit Γ₁ Γ₃
+  := (h12_3.s12_3_31 h12).comm
+
+abbrev Ctx?.SSplit.c12_34_123 {Γ₁₂₃₄ Γ₁₂ Γ₃₄ Γ₃ Γ₄ : Ctx? α ε}
+  (h12_34 : Γ₁₂₃₄.SSplit Γ₁₂ Γ₃₄) (h34 : Γ₃₄.SSplit Γ₃ Γ₄)
+  : Ctx? α ε := h12_34.c1_23_12 h34
+
+abbrev Ctx?.SSplit.s12_34_123_4 {Γ₁₂₃₄ Γ₁₂ Γ₃₄ Γ₃ Γ₄ : Ctx? α ε}
+  (h12_34 : Γ₁₂₃₄.SSplit Γ₁₂ Γ₃₄) (h34 : Γ₃₄.SSplit Γ₃ Γ₄)
+  : Γ₁₂₃₄.SSplit (h12_34.c12_34_123 h34) Γ₄ := h12_34.s1_23_12_3 h34
+
+abbrev Ctx?.SSplit.s12_34_12_3 {Γ₁₂₃₄ Γ₁₂ Γ₃₄ Γ₃ Γ₄ : Ctx? α ε}
+  (h12_34 : Γ₁₂₃₄.SSplit Γ₁₂ Γ₃₄) (h34 : Γ₃₄.SSplit Γ₃ Γ₄)
+  : (h12_34.c12_34_123 h34).SSplit Γ₁₂ Γ₃ := h12_34.s1_23_12 h34
+
+abbrev Ctx?.SSplit.c12_34_13 {Γ₁₂₃₄ Γ₁₂ Γ₃₄ Γ₃ Γ₄ : Ctx? α ε}
+  (h12_34 : Γ₁₂₃₄.SSplit Γ₁₂ Γ₃₄) (h12 : Γ₁₂.SSplit Γ₁ Γ₂) (h34 : Γ₃₄.SSplit Γ₃ Γ₄)
+  : Ctx? α ε := (h12_34.s12_34_12_3 h34).c12_3_13 h12
+
+abbrev Ctx?.SSplit.s12_34_13 {Γ₁₂₃₄ Γ₁₂ Γ₃₄ Γ₃ Γ₄ : Ctx? α ε}
+  (h12_34 : Γ₁₂₃₄.SSplit Γ₁₂ Γ₃₄) (h12 : Γ₁₂.SSplit Γ₁ Γ₂) (h34 : Γ₃₄.SSplit Γ₃ Γ₄)
+  : (h12_34.c12_34_13 h12 h34).SSplit Γ₁ Γ₃ := (h12_34.s12_34_12_3 h34).s12_3_13 h12
+
+abbrev Ctx?.SSplit.s12_34_13_2 {Γ₁₂₃₄ Γ₁₂ Γ₃₄ Γ₃ Γ₄ : Ctx? α ε}
+  (h12_34 : Γ₁₂₃₄.SSplit Γ₁₂ Γ₃₄) (h12 : Γ₁₂.SSplit Γ₁ Γ₂) (h34 : Γ₃₄.SSplit Γ₃ Γ₄)
+  : (h12_34.c12_34_123 h34).SSplit (h12_34.c12_34_13 h12 h34) Γ₂
+  := (h12_34.s12_34_12_3 h34).s12_3_13_2 h12
+
+abbrev Ctx?.SSplit.c12_34_24 {Γ₁₂₃₄ Γ₁₂ Γ₃₄ Γ₃ Γ₄ : Ctx? α ε}
+  (h12_34 : Γ₁₂₃₄.SSplit Γ₁₂ Γ₃₄) (h12 : Γ₁₂.SSplit Γ₁ Γ₂) (h34 : Γ₃₄.SSplit Γ₃ Γ₄)
+  : Ctx? α ε
+  := (h12_34.s12_34_123_4 h34).c12_3_23 (h12_34.s12_34_13_2 h12 h34)
+
+abbrev Ctx?.SSplit.s12_34_13_24 {Γ₁₂₃₄ Γ₁₂ Γ₃₄ Γ₃ Γ₄ : Ctx? α ε}
+  (h12_34 : Γ₁₂₃₄.SSplit Γ₁₂ Γ₃₄) (h12 : Γ₁₂.SSplit Γ₁ Γ₂) (h34 : Γ₃₄.SSplit Γ₃ Γ₄)
+  : Γ₁₂₃₄.SSplit (h12_34.c12_34_13 h12 h34) (h12_34.c12_34_24 h12 h34)
+  := (h12_34.s12_34_123_4 h34).s12_3_1_23 (h12_34.s12_34_13_2 h12 h34)
+
+abbrev Ctx?.SSplit.s12_34_24 {Γ₁₂₃₄ Γ₁₂ Γ₃₄ Γ₃ Γ₄ : Ctx? α ε}
+  (h12_34 : Γ₁₂₃₄.SSplit Γ₁₂ Γ₃₄) (h12 : Γ₁₂.SSplit Γ₁ Γ₂) (h34 : Γ₃₄.SSplit Γ₃ Γ₄)
+  : (h12_34.c12_34_24 h12 h34).SSplit Γ₂ Γ₄
+  := (h12_34.s12_34_123_4 h34).s12_3_23 (h12_34.s12_34_13_2 h12 h34)
+
+variable [PartialOrder ε]
+
+
+inductive Var?.Split : Var? α ε → Var? α ε → Var? α ε → Type _
+  | left {v w} (h : v ≤ w) (e) : Split v w ⟨v.ty, 0, e⟩
+  | right {v w} (h : v ≤ w) (e) : Split v ⟨v.ty, 0, e⟩ w
+  | sboth {u v w} : u.scopy → u ≤ v → u ≤ w → Split u v w
+
+inductive Ctx?.Split : Ctx? α ε → Ctx? α ε → Ctx? α ε → Type _ where
+  | nil : Ctx?.Split .nil .nil .nil
+  | cons {Γ Δ Ξ v l r} (h : Split Γ Δ Ξ) (hvw : v.Split l r)
+    : Split (Ctx?.cons Γ v) (Ctx?.cons Δ l) (Ctx?.cons Ξ r)
+
+def Var?.SSplit.toSplit {u v w : Var? α ε} (h : u.SSplit v w) : u.Split v w := match h with
+  | Var?.SSplit.left _ => Var?.Split.left (le_refl _) _
+  | Var?.SSplit.right _ => Var?.Split.right (le_refl _) _
+  | Var?.SSplit.sboth hu => Var?.Split.sboth hu (le_refl _) (le_refl _)
+
+def Ctx?.SSplit.toSplit {Γ Δ Ξ : Ctx? α ε} : Ctx?.SSplit Γ Δ Ξ → Ctx?.Split Γ Δ Ξ
+  | .nil => .nil
+  | .cons h hvw => .cons h.toSplit hvw.toSplit
+
+def Var?.SSplit.wk {u' u v w : Var? α ε} (ρ : u' ≤ u) (σ : u.SSplit v w) :
+  u'.SSplit (σ.wkLeft u') (σ.wkRight u') := match u, σ with
+  | ⟨A, (q : Quant), e⟩, .left _ => .left _
+  | ⟨A, (q : Quant), e⟩, .right _ => .right _
+  | ⟨A, 0, e⟩, .left _ | ⟨A, 0, e⟩, .right _ => .right _
+  | ⟨A, (q : Quant), e⟩, .sboth h => .sboth (h.anti ρ)
+
+@[simp]
+theorem Var?.SSplit.wk_left_quant {u' : Var? α ε} {A : Ty α} {q : Quant} {e : ε}
+  (ρ : u' ≤ ⟨A, q, e⟩) : (SSplit.left ⟨A, q, e⟩).wk ρ = .left u' := rfl
+
+@[simp]
+theorem Var?.SSplit.wk_right_quant {u' : Var? α ε} {A : Ty α} {q : Quant} {e : ε}
+  (ρ : u' ≤ ⟨A, q, e⟩) : (SSplit.right ⟨A, q, e⟩).wk ρ = .right u' := rfl
+
+@[simp]
+theorem Var?.SSplit.wk_left_zero {u' : Var? α ε} {A : Ty α} {e : ε}
+  (ρ : u' ≤ ⟨A, 0, e⟩) : (SSplit.left ⟨A, 0, e⟩).wk ρ = .right u' := rfl
+
+@[simp]
+theorem Var?.SSplit.wk_right_zero {u' : Var? α ε} {A : Ty α} {e : ε}
+  (ρ : u' ≤ ⟨A, 0, e⟩) : (SSplit.right ⟨A, 0, e⟩).wk ρ = .right u' := rfl
+
+@[simp]
+theorem Var?.SSplit.wk_sboth_quant {u' : Var? α ε} {A : Ty α} {q : Quant} {e : ε}
+  (ρ : u' ≤ ⟨A, q, e⟩) (h : (Var?.mk A q e).scopy)
+  : (SSplit.sboth h).wk ρ = SSplit.sboth (h.anti ρ) := rfl
+
+@[simp]
+theorem Var?.SSplit.leftWk {u' u v w : Var? α ε} (ρ : u' ≤ u) (σ : u.SSplit v w)
+  : (σ.wkLeft u') ≤ v := by cases u with | mk A q e =>
+    cases q using EQuant.casesZero <;> cases σ <;> first | exact ρ | exact (erase_mono ρ)
+
+@[simp]
+theorem Var?.SSplit.rightWk {u' u v w : Var? α ε} (ρ : u' ≤ u) (σ : u.SSplit v w)
+  : (σ.wkRight u') ≤ w := by cases u with | mk A q e =>
+    cases q using EQuant.casesZero <;> cases σ <;> first | exact ρ | exact (erase_mono ρ)
+
+def Var?.SSplit.wk' {u' u v w : Var? α ε} (ρ : u' ≤ u) (σ : u.SSplit v w) :
+  u'.SSplit (σ.wkLeft' u') (σ.wkRight' u') := match u, σ with
+  | ⟨A, (q : Quant), e⟩, .left _ => .left _
+  | ⟨A, (q : Quant), e⟩, .right _ => .right _
+  | ⟨A, 0, e⟩, .left _ | ⟨A, 0, e⟩, .right _ => .left _
+  | ⟨A, (q : Quant), e⟩, .sboth h => .sboth (h.anti ρ)
+
+@[simp]
+theorem Var?.SSplit.wk_left_quant' {u' : Var? α ε} {A : Ty α} {q : Quant} {e : ε}
+  (ρ : u' ≤ ⟨A, q, e⟩) : (SSplit.left ⟨A, q, e⟩).wk' ρ = .left u' := rfl
+
+@[simp]
+theorem Var?.SSplit.wk_right_quant' {u' : Var? α ε} {A : Ty α} {q : Quant} {e : ε}
+  (ρ : u' ≤ ⟨A, q, e⟩) : (SSplit.right ⟨A, q, e⟩).wk' ρ = .right u' := rfl
+
+@[simp]
+theorem Var?.SSplit.wk_left_zero' {u' : Var? α ε} {A : Ty α} {e : ε}
+  (ρ : u' ≤ ⟨A, 0, e⟩) : (SSplit.left ⟨A, 0, e⟩).wk' ρ = .left u' := rfl
+
+@[simp]
+theorem Var?.SSplit.wk_right_zero' {u' : Var? α ε} {A : Ty α} {e : ε}
+  (ρ : u' ≤ ⟨A, 0, e⟩) : (SSplit.right ⟨A, 0, e⟩).wk' ρ = .left u' := rfl
+
+@[simp]
+theorem Var?.SSplit.wk_sboth_quant' {u' : Var? α ε} {A : Ty α} {q : Quant} {e : ε}
+  (ρ : u' ≤ ⟨A, q, e⟩) (h : (Var?.mk A q e).scopy)
+  : (SSplit.sboth h).wk' ρ = SSplit.sboth (h.anti ρ) := rfl
+
+@[simp]
+theorem Var?.SSplit.leftWk' {u' u v w : Var? α ε} (ρ : u' ≤ u) (σ : u.SSplit v w)
+  : (σ.wkLeft' u') ≤ v := by cases u with | mk A q e =>
+    cases q using EQuant.casesZero <;> cases σ <;> first | exact ρ | exact (erase_mono ρ)
+
+@[simp]
+theorem Var?.SSplit.rightWk' {u' u v w : Var? α ε} (ρ : u' ≤ u) (σ : u.SSplit v w)
+  : (σ.wkRight' u') ≤ w := by cases u with | mk A q e =>
+    cases q using EQuant.casesZero <;> cases σ <;> first | exact ρ | exact (erase_mono ρ)
+
+@[simp]
+def Ctx?.SSplit.wkLeft {Γ' Γ Δ Ξ : Ctx? α ε}
+  : Γ'.Wk Γ → Γ.SSplit Δ Ξ → Ctx? α ε
+  | .nil, _ => .nil
+  | .skip (v := v) ρ _, σ => (wkLeft ρ σ).cons v.erase
+  | .cons (v := v) ρ _, .cons σ hlr => (wkLeft ρ σ).cons (hlr.wkLeft v)
+
+@[simp]
+def Ctx?.SSplit.wkRight {Γ' Γ Δ Ξ : Ctx? α ε}
+  : Γ'.Wk Γ → Γ.SSplit Δ Ξ → Ctx? α ε
+  | .nil, _ => .nil
+  | .skip (v := v) ρ _, σ => (wkRight ρ σ).cons v
+  | .cons (v := v) ρ _, .cons σ hlr => (wkRight ρ σ).cons (hlr.wkRight v)
+
+@[simp]
+def Ctx?.SSplit.leftWk {Γ' Γ Δ Ξ : Ctx? α ε}
+  : (ρ : Γ'.Wk Γ) → (σ : Γ.SSplit Δ Ξ) → (σ.wkLeft ρ).Wk Δ
+  | .nil, .nil => .nil
+  | .skip ρ _, σ => .skip (σ.leftWk ρ) inferInstance
+  | .cons ρ hvw, .cons σ hlr => .cons (σ.leftWk ρ) (hlr.leftWk hvw)
+
+@[simp]
+def Ctx?.SSplit.rightWk {Γ' Γ Δ Ξ : Ctx? α ε}
+  : (ρ : Γ'.Wk Γ) → (σ : Γ.SSplit Δ Ξ) → (σ.wkRight ρ).Wk Ξ
+  | .nil, .nil => .nil
+  | .skip ρ _, σ => .skip (σ.rightWk ρ) inferInstance
+  | .cons ρ hvw, .cons σ hlr => .cons (σ.rightWk ρ) (hlr.rightWk hvw)
+
+@[simp]
+theorem Ctx?.SSplit.ix_leftWk {Γ' Γ Δ Ξ : Ctx? α ε} (ρ : Γ'.Wk Γ) (σ : Γ.SSplit Δ Ξ)
+  : (σ.leftWk ρ).ix = ρ := by
+    induction ρ generalizing Δ Ξ <;> cases σ <;> simp [*]
+
+theorem Ctx?.SSplit.leftWk_applied {Γ' Γ Δ Ξ : Ctx? α ε} (ρ : Γ'.Wk Γ) (σ : Γ.SSplit Δ Ξ) (i : ℕ)
+  : (σ.leftWk ρ) i = ρ i := by simp
+
+@[simp]
+theorem Ctx?.SSplit.ix_rightWk {Γ' Γ Δ Ξ : Ctx? α ε} (ρ : Γ'.Wk Γ) (σ : Γ.SSplit Δ Ξ)
+  : (σ.rightWk ρ).ix = ρ := by
+    induction ρ generalizing Δ Ξ <;> cases σ <;> simp [*]
+
+theorem Ctx?.SSplit.rightWk_applied {Γ' Γ Δ Ξ : Ctx? α ε} (ρ : Γ'.Wk Γ) (σ : Γ.SSplit Δ Ξ) (i : ℕ)
+  : (σ.rightWk ρ) i = ρ i := by simp
+
+@[simp]
+def Ctx?.SSplit.wk {Γ' Γ Δ Ξ : Ctx? α ε}
+  : (ρ : Γ'.Wk Γ) → (σ : Γ.SSplit Δ Ξ) → Γ'.SSplit (σ.wkLeft ρ) (σ.wkRight ρ)
+  | .nil, .nil => .nil
+  | .skip (v := ⟨A, q, e⟩) ρ _, σ => .cons (σ.wk ρ) (.right ..)
+  | .cons ρ hvw, .cons σ hlr => .cons (σ.wk ρ) (hlr.wk hvw)
+
+theorem Var?.SSplit.wkLeft_copy
+  {u' u v w : Var? α ε} (ρ : u' ≤ u) (σ : u.SSplit v w) [hv : v.copy]
+  : (σ.wkLeft u').copy := by cases u with | mk A q e =>
+    cases q using EQuant.casesZero with
+    | zero => cases σ <;> simp
+    | rest q => cases σ <;> simp <;> apply copy.anti (hw := _) ρ <;> simp [*]
+
+theorem Var?.SSplit.wkLeft_del
+  {u' u v w : Var? α ε} (ρ : u' ≤ u) (σ : u.SSplit v w) [hv : v.del]
+  : (σ.wkLeft u').del := by cases u with | mk A q e =>
+    cases q using EQuant.casesZero with
+    | zero => cases σ <;> simp
+    | rest q => cases σ <;> simp <;> apply del.anti (hw := _) ρ <;> simp [*]
+
+instance Ctx?.SSplit.wkLeft_del
+  {Γ' Γ Δ Ξ : Ctx? α ε} (ρ : Γ'.Wk Γ) (σ : Γ.SSplit Δ Ξ) [hΔ : Δ.del] : (σ.wkLeft ρ).del
+  := by induction ρ generalizing Δ Ξ with
+  | nil => simp
+  | skip ρ hv I => simp [*]
+  | cons ρ hvw I =>
+    cases σ; have _ := hΔ.head; have _ := hΔ.tail;
+    simp [wkLeft, cons_del_iff, Var?.SSplit.wkLeft_del, *]
+
+-- Since all unused variables go on the right, we have the following useful theorems:
+instance Ctx?.SSplit.wkLeft_copy
+  {Γ' Γ Δ Ξ : Ctx? α ε} (ρ : Γ'.Wk Γ) (σ : Γ.SSplit Δ Ξ) [hΔ : Δ.copy] : (σ.wkLeft ρ).copy
+  := by induction ρ generalizing Δ Ξ with
+  | nil => simp
+  | skip ρ hv I => simp [*]
+  | cons ρ hvw I =>
+    cases σ; have _ := hΔ.head; have _ := hΔ.tail;
+    simp [wkLeft, cons_copy_iff, Var?.SSplit.wkLeft_copy, *]
+
+@[simp]
+def Ctx?.SSplit.wkLeft' {Γ' Γ Δ Ξ : Ctx? α ε}
+  : Γ'.Wk Γ → Γ.SSplit Δ Ξ → Ctx? α ε
+  | .nil, _ => .nil
+  | .skip (v := v) ρ _, σ => (wkLeft' ρ σ).cons v
+  | .cons (v := v) ρ _, .cons σ hlr => (wkLeft' ρ σ).cons (hlr.wkLeft' v)
+
+@[simp]
+def Ctx?.SSplit.wkRight' {Γ' Γ Δ Ξ : Ctx? α ε}
+  : Γ'.Wk Γ → Γ.SSplit Δ Ξ → Ctx? α ε
+  | .nil, _ => .nil
+  | .skip (v := v) ρ _, σ => (wkRight' ρ σ).cons v.erase
+  | .cons (v := v) ρ _, .cons σ hlr => (wkRight' ρ σ).cons (hlr.wkRight' v)
+
+@[simp]
+def Ctx?.SSplit.leftWk' {Γ' Γ Δ Ξ : Ctx? α ε}
+  : (ρ : Γ'.Wk Γ) → (σ : Γ.SSplit Δ Ξ) → (σ.wkLeft' ρ).Wk Δ
+  | .nil, .nil => .nil
+  | .skip ρ _, σ => .skip (σ.leftWk' ρ) inferInstance
+  | .cons ρ hvw, .cons σ hlr => .cons (σ.leftWk' ρ) (hlr.leftWk' hvw)
+
+@[simp]
+def Ctx?.SSplit.rightWk' {Γ' Γ Δ Ξ : Ctx? α ε}
+  : (ρ : Γ'.Wk Γ) → (σ : Γ.SSplit Δ Ξ) → (σ.wkRight' ρ).Wk Ξ
+  | .nil, .nil => .nil
+  | .skip ρ _, σ => .skip (σ.rightWk' ρ) inferInstance
+  | .cons ρ hvw, .cons σ hlr => .cons (σ.rightWk' ρ) (hlr.rightWk' hvw)
+
+@[simp]
+theorem Ctx?.SSplit.ix_leftWk' {Γ' Γ Δ Ξ : Ctx? α ε} (ρ : Γ'.Wk Γ) (σ : Γ.SSplit Δ Ξ)
+  : (σ.leftWk' ρ).ix = ρ := by
+    induction ρ generalizing Δ Ξ <;> cases σ <;> simp [*]
+
+theorem Ctx?.SSplit.leftWk_applied' {Γ' Γ Δ Ξ : Ctx? α ε} (ρ : Γ'.Wk Γ) (σ : Γ.SSplit Δ Ξ) (i : ℕ)
+  : (σ.leftWk ρ) i = ρ i := by simp
+
+@[simp]
+theorem Ctx?.SSplit.ix_rightWk' {Γ' Γ Δ Ξ : Ctx? α ε} (ρ : Γ'.Wk Γ) (σ : Γ.SSplit Δ Ξ)
+  : (σ.rightWk ρ).ix = ρ := by
+    induction ρ generalizing Δ Ξ <;> cases σ <;> simp [*]
+
+theorem Ctx?.SSplit.rightWk_applied' {Γ' Γ Δ Ξ : Ctx? α ε} (ρ : Γ'.Wk Γ) (σ : Γ.SSplit Δ Ξ) (i : ℕ)
+  : (σ.rightWk ρ) i = ρ i := by simp
+
+@[simp]
+def Ctx?.SSplit.wk' {Γ' Γ Δ Ξ : Ctx? α ε}
+  : (ρ : Γ'.Wk Γ) → (σ : Γ.SSplit Δ Ξ) → Γ'.SSplit (σ.wkLeft' ρ) (σ.wkRight' ρ)
+  | .nil, .nil => .nil
+  | .skip (v := ⟨A, q, e⟩) ρ _, σ => .cons (σ.wk' ρ) (.left ..)
+  | .cons ρ hvw, .cons σ hlr => .cons (σ.wk' ρ) (hlr.wk' hvw)
+
+theorem Var?.SSplit.wkRight_copy'
+  {u' u v w : Var? α ε} (ρ : u' ≤ u) (σ : u.SSplit v w) [hw : w.copy]
+  : (σ.wkRight' u').copy := by cases u with | mk A q e =>
+    cases q using EQuant.casesZero with
+    | zero => cases σ <;> simp
+    | rest q => cases σ <;> simp <;> apply copy.anti (hw := _) ρ <;> simp [*]
+
+theorem Var?.SSplit.wkLeft_del'
+  {u' u v w : Var? α ε} (ρ : u' ≤ u) (σ : u.SSplit v w) [hv : v.del]
+  : (σ.wkLeft u').del := by cases u with | mk A q e =>
+    cases q using EQuant.casesZero with
+    | zero => cases σ <;> simp
+    | rest q => cases σ <;> simp <;> apply del.anti (hw := _) ρ <;> simp [*]
+
+instance Ctx?.SSplit.wkLeft_del'
+  {Γ' Γ Δ Ξ : Ctx? α ε} (ρ : Γ'.Wk Γ) (σ : Γ.SSplit Δ Ξ) [hΔ : Δ.del] : (σ.wkLeft ρ).del
+  := by induction ρ generalizing Δ Ξ with
+  | nil => simp
+  | skip ρ hv I => simp [*]
+  | cons ρ hvw I =>
+    cases σ; have _ := hΔ.head; have _ := hΔ.tail;
+    simp [wkLeft, cons_del_iff, Var?.SSplit.wkLeft_del, *]
+
+-- Since all unused variables go on the left, we have the following useful theorem:
+instance Ctx?.SSplit.wkRight_copy'
+  {Γ' Γ Δ Ξ : Ctx? α ε} (ρ : Γ'.Wk Γ) (σ : Γ.SSplit Δ Ξ) [hΞ : Ξ.copy] : (σ.wkRight' ρ).copy
+  := by induction ρ generalizing Δ Ξ with
+  | nil => simp
+  | skip ρ hv I => simp[*]
+  | cons ρ hvw I =>
+    cases σ; have _ := hΞ.head; have _ := hΞ.tail;
+    simp [wkLeft, cons_copy_iff, Var?.SSplit.wkRight_copy', *]
+
+def Ctx?.erase_right : (Γ : Ctx? α ε) → Γ.SSplit Γ Γ.erase
+  | .nil => .nil
+  | .cons Γ v => .cons Γ.erase_right (.left v)
+
+def Ctx?.erase_left : (Γ : Ctx? α ε) → Γ.SSplit Γ.erase Γ
+  | .nil => .nil
+  | .cons Γ v => .cons Γ.erase_left (.right v)
+
+theorem Var?.SSplit.wkLeft_quant
+  {u' u v w : Var? α ε} (ρ : u' ≤ u) (σ : u.SSplit v w)
+  : quant v ≤ quant (σ.wkLeft u') := by cases u with | mk A q e =>
+    cases q using EQuant.casesZero with
+    | zero => cases σ <;> rfl
+    | rest q =>
+      cases σ <;> simp <;>
+      cases u' with | mk A' q' e' =>
+      cases q' using EQuant.casesZero with
+      | zero => cases ρ.q using EQuant.le.casesLE
+      | rest q' =>
+        have h := ρ.q; simp only [quant] at h;
+        cases ρ.ty; simp [quant]; apply inf_le_of_left_le; rw [<-EQuant.coe_le_coe]; exact ρ.q
+
+theorem Var?.SSplit.wkRight_quant'
+  {u' u v w : Var? α ε} (ρ : u' ≤ u) (σ : u.SSplit v w)
+  : quant w ≤ quant (σ.wkRight' u') := by cases u with | mk A q e =>
+    cases q using EQuant.casesZero with
+    | zero => cases σ <;> rfl
+    | rest q =>
+      cases σ <;> simp <;>
+      cases u' with | mk A' q' e' =>
+      cases q' using EQuant.casesZero with
+      | zero => cases ρ.q using EQuant.le.casesLE
+      | rest q' =>
+        have h := ρ.q; simp only [quant] at h;
+        cases ρ.ty; simp [quant]; apply inf_le_of_left_le; rw [<-EQuant.coe_le_coe]; exact ρ.q
+
+theorem Ctx?.SSplit.wkLeft_quant
+  {Γ' Γ Δ Ξ : Ctx? α ε} (ρ : Γ'.Wk Γ) (σ : Γ.SSplit Δ Ξ)
+  : quant Δ ≤ quant (σ.wkLeft ρ) := by induction ρ generalizing Δ Ξ with
+  | cons =>
+    cases σ; simp only [quant_cons, wkLeft]
+    apply inf_le_inf
+    apply_assumption
+    apply Var?.SSplit.wkLeft_quant
+    assumption
+  | _ => simp [*]
+
+theorem Ctx?.SSplit.wkRight_quant'
+  {Γ' Γ Δ Ξ : Ctx? α ε} (ρ : Γ'.Wk Γ) (σ : Γ.SSplit Δ Ξ)
+  : quant Ξ ≤ quant (σ.wkRight' ρ) := by induction ρ generalizing Δ Ξ with
+  | cons =>
+    cases σ; simp only [quant_cons, wkRight']
+    apply inf_le_inf
+    apply_assumption
+    apply Var?.SSplit.wkRight_quant'
+    assumption
+  | _ => simp [*]
+
+@[simp]
+def Var?.SSplit.leftCtx {u v w : Var? α ε} : u.SSplit v w → Ctx? α ε → Ctx? α ε
+  | .left _, Γ | .sboth _, Γ => Γ
+  | .right _, Γ => Γ.erase
+
+@[simp]
+def Var?.SSplit.rightCtx {u v w : Var? α ε} : u.SSplit v w → Ctx? α ε → Ctx? α ε
+  | .left _, Γ => Γ.erase
+  | .right _, Γ | .sboth _, Γ => Γ
+
+def Var?.SSplit.lift {u v w : Var? α ε} (Γ : Ctx? α ε) (hΓ : quant u ≤ quant Γ)
+  : (h : u.SSplit v w) → Γ.SSplit (h.leftCtx Γ) (h.rightCtx Γ)
+  | .left _ => Γ.erase_right
+  | .right _ => Γ.erase_left
+  | .sboth h => Γ.both (hΓ := ⟨le_trans h.copy.copy_le_quant hΓ⟩)
